Verify formula for counting models of a decomposable formula

lean4/ProofChecker/ProofChecker/CountModels.lean
@@ -15,13 +15,13 @@ variable {ν : Type u} [DecidableEq ν]
 /-- The unique evaluation function on formulas which extends `τ`. -/
 @[simp]
 def vars : PropForm ν → Finset ν
-  | var x => {x}
-  | tr => ∅
-  | fls => ∅
-  | neg φ => vars φ
-  | conj φ₁ φ₂ => vars φ₁ ∪ vars φ₂
-  | disj φ₁ φ₂ => vars φ₁ ∪ vars φ₂
-  | impl φ₁ φ₂ => vars φ₁ ∪ vars φ₂
+  | var x        => {x}
+  | tr           => ∅
+  | fls          => ∅
+  | neg φ        => vars φ
+  | conj φ₁ φ₂   => vars φ₁ ∪ vars φ₂
+  | disj φ₁ φ₂   => vars φ₁ ∪ vars φ₂
+  | impl φ₁ φ₂   => vars φ₁ ∪ vars φ₂
   | biImpl φ₁ φ₂ => vars φ₁ ∪ vars φ₂
 
 theorem eval_ext {φ : PropForm ν} {v₁ v₂ : PropAssignment ν} (h : ∀ x ∈ φ.vars, v₁ x = v₂ x) :
@@ -42,8 +42,8 @@ def decomposable [DecidableEq ν]: PropForm ν → Prop
   | fls        => True
   | var _      => True
   | neg φ      => φ.decomposable
-  | disj φ₁ φ₂ => φ₁.decomposable ∧ φ₂.decomposable ∧ ∀ v, ¬ (φ₁.eval v ∧ φ₂.eval v)
-  | conj φ₁ φ₂ => φ₁.decomposable ∧ φ₂.decomposable ∧ (φ₁.vars ∩ φ₂.vars = ∅)
+  | disj φ ψ   => φ.decomposable ∧ ψ.decomposable ∧ ∀ v, ¬ (φ.eval v ∧ ψ.eval v)
+  | conj φ ψ   => φ.decomposable ∧ ψ.decomposable ∧ (φ.vars ∩ ψ.vars = ∅)
   | impl _ _   => False
   | biImpl _ _ => False
 
@@ -52,8 +52,8 @@ def countModels (s : Finset ν) : PropForm ν → Nat
   | fls        => 0
   | var _      => 2^(card s - 1)
   | neg φ      => 2^(card s) - φ.countModels s
-  | disj φ₁ φ₂ => φ₁.countModels s + φ₂.countModels s
-  | conj φ₁ φ₂ => (φ₁.countModels s) * (φ₂.countModels s) / 2^(card s)
+  | disj φ ψ   => φ.countModels s + ψ.countModels s
+  | conj φ ψ   => φ.countModels s * ψ.countModels s / 2^(card s)
   | impl _ _   => 0
   | biImpl _ _ => 0
 
@@ -65,7 +65,10 @@ Propositional assignments and their restrictions to finsets.
 
 namespace PropAssignment
 
-def defined_on (v : PropAssignment ν) (s : Finset ν) : Prop := ∀ ⦃n⦄, n ∉ s → v n = false
+def defined_on (v : PropAssignment ν) (s : Finset ν) : Prop := ∀ ⦃x⦄, x ∉ s → v x = false
+
+theorem eq_false_of_defined_on {v : PropAssignment ν} {s : Finset ν} {x : ν}
+    (h : v.defined_on s) (h' : ¬ x ∈ s) : v x = false := h h'
 
 theorem defined_on_mono {v : PropAssignment ν} {s t : Finset ν} (h : s ⊆ t) :
     v.defined_on s → v.defined_on t :=
@@ -108,13 +111,19 @@ theorem toPropAssignment_eq_false {x : ν} (s : Finset ν) :
     s.toPropAssignment x = false ↔ x ∉ s := by
   simp [←toPropAssignment_eq_true]
 
+theorem injective_toPropAssignment : Function.Injective (@toPropAssignment ν _) := by
+  intro s1 s2 heq
+  ext x
+  have := congr_fun heq x
+  rw [←s1.toPropAssignment_eq_true, this, s2.toPropAssignment_eq_true]
+
 end Finset
 
 /-
 Models of a propositional formula over a set of variables.
 
-Note: we don't intend to use this theory computationally, so we use classical logic to declare decidable equality
-on `PropAssignment ν`.
+Note: we don't intend to use this theory computationally, so we use classical logic to declare
+decidable equality on `PropAssignment ν`.
 -/
 
 variable [DecidableEq ν]
@@ -124,24 +133,26 @@ noncomputable instance : DecidableEq (PropAssignment ν) := fun _ _ => Classical
 namespace Finset
 
 noncomputable def assignments (s : Finset ν) : Finset (PropAssignment ν) :=
-  s.powerset.image (fun (t : Finset ν) (v : ν) => if v ∈ t then true else false)
+  s.powerset.image toPropAssignment
 
-theorem mem_assignments (s : Finset ν) (v : PropAssignment ν) : v ∈ assignments s ↔ v.defined_on s := by
+@[simp] theorem mem_assignments (s : Finset ν) (v : PropAssignment ν) :
+    v ∈ assignments s ↔ v.defined_on s := by
+  simp only [assignments, mem_image, mem_powerset]
   constructor
-  . intro (h : v ∈ assignments s) i hnis
-    rcases mem_image.mp h with ⟨t, ⟨htpows, rfl⟩⟩
-    simp only [ite_eq_right_iff]
-    rw [mem_powerset] at htpows
-    intro (hit : i ∈ t)
-    exact hnis (htpows hit)
+  . rintro ⟨t, ht1, rfl⟩ x hx
+    rw [toPropAssignment_eq_false]
+    intro h; exact hx (ht1 h)
   . intro h
-    rw [assignments, mem_image]
     use s.filter (v . = true)
-    constructor
-    . rw [mem_powerset]; apply filter_subset
-    . ext i; split
-      . simp_all [mem_filter]
-      . by_cases h' : i ∈ s <;> simp_all [PropAssignment.defined_on]
+    simp only [filter_subset, true_and]
+    ext x
+    simp only [toPropAssignment, mem_filter]
+    by_cases hx : x ∈ s
+    . cases (v x) <;> simp [hx]
+    . simp [hx, h hx]
+
+theorem card_assignments (s : Finset ν) : card (assignments s) = 2^(card s) := by
+  rw [assignments, card_image_of_injective _ injective_toPropAssignment, card_powerset]
 
 end Finset
 
@@ -150,7 +161,78 @@ namespace PropForm
 noncomputable def models (φ : PropForm ν) (s : Finset ν) := s.assignments.filter (φ.eval .)
 
 @[simp] theorem mem_models {φ : PropForm ν} {s : Finset ν} (v : PropAssignment ν) :
-    v ∈ φ.models s ↔ v.defined_on s ∧ φ.eval v = true := by rw [models, mem_filter, mem_assignments]
+    v ∈ φ.models s ↔ v.defined_on s ∧ φ.eval v = true :=
+  by rw [models, mem_filter, mem_assignments]
+
+@[simp] theorem card_models_tr (s : Finset ν) : card ((tr : PropForm ν).models s) = 2^(card s) := by
+  simp [models, card_assignments]
+
+@[simp] theorem card_models_fls (s : Finset ν) : card ((fls : PropForm ν).models s) = 0 := by
+  simp [models, card_assignments]
+
+@[simp] theorem card_models_var {x : ν} {s : Finset ν} (hxs : x ∈ s) :
+    card ((var x).models s) = 2^(card s - 1) := by
+  let f (v : PropAssignment ν) : PropAssignment ν := fun x' => if x' = x then true else v x'
+  have h1 : (var x).models s = (assignments (s.erase x)).image f := by
+    ext v; simp only [mem_models, eval, mem_image]
+    constructor
+    . intro ⟨hvdef, hvx⟩
+      use fun x' => if x' = x then false else v x'
+      constructor
+      . rw [mem_assignments]
+        intro x' hx'
+        rw [mem_erase, not_and] at hx'; dsimp
+        split <;> simp_all [v.eq_false_of_defined_on hvdef]
+      . ext x'
+        split <;> simp_all [v.eq_false_of_defined_on hvdef]
+    . rintro ⟨v', hv', rfl⟩
+      rw [mem_assignments] at hv'
+      constructor
+      . intro x' hx'
+        have : x' ≠ x := by rintro rfl; contradiction
+        dsimp; rw [if_neg this, v'.eq_false_of_defined_on hv']
+        rw [mem_erase, not_and_or]; right; exact hx'
+      . simp
+  have h2 : Set.InjOn f (assignments (s.erase x)) := by
+    intro v1 hv1 v2 hv2 heq
+    simp only [mem_coe, mem_assignments] at hv1 hv2
+    ext x'
+    have := congr_fun heq x'
+    clear h1 heq; revert f; dsimp
+    split
+    . simp_all
+      have : x ∉ erase s x := by simp [mem_erase]
+      rw [hv1 this, hv2 this]
+    . exact id
+  rw [h1, card_image_of_injOn h2, card_assignments, card_erase_of_mem hxs]
+
+@[simp] theorem card_models_disj_disjoint {φ ψ : PropForm ν} (s : Finset ν)
+      (h : ∀ v, ¬ (φ.eval v ∧ ψ.eval v)) :
+    card ((φ.disj ψ).models s) = card (φ.models s) + card (ψ.models s) := by
+  have : (φ.disj ψ).models s = (φ.models s) ∪ (ψ.models s) := by
+    ext v; simp only [mem_models, eval, Bool.or_eq_true, mem_union]
+    rw [and_or_left]
+  rw [this, card_disjoint_union]
+  rw [disjoint_iff_ne]
+  rintro v hv1 _ hv2 rfl
+  apply h v
+  rw [mem_models] at hv1 hv2
+  rw [hv1.2, hv2.2]; simp
+
+@[simp] theorem card_models_neg (φ : PropForm ν) (s : Finset ν) :
+    card (φ.neg.models s) = 2^(card s) - card (φ.models s) := by
+  symm; apply Nat.sub_eq_of_eq_add
+  rw [←card_assignments s]
+  have : assignments s = φ.neg.models s ∪ φ.models s := by
+    ext v; simp only [mem_assignments, mem_union, mem_models, eval, Bool.bnot_eq_to_not_eq,
+      Bool.not_eq_true]
+    rw [←and_or_left]; cases (eval v φ) <;> simp
+  rw [this, card_disjoint_union]
+  rw [disjoint_iff_ne]
+  rintro v hv1 _ hv2 rfl
+  rw [mem_models] at hv2
+  rw [mem_models, eval, hv2.2] at hv1
+  simp at hv1
 
 theorem card_models_vars {φ : PropForm ν} {s : Finset ν} (h : φ.vars ⊆ s) :
     card (φ.models s) = card (φ.models φ.vars) * 2^(card s - card φ.vars) := by
@@ -184,8 +266,8 @@ theorem card_models_vars {φ : PropForm ν} {s : Finset ν} (h : φ.vars ⊆ s) 
           by_cases hxs : x ∈ s <;> split <;> simp_all [@hvdef x]
   have h2 : Set.InjOn f <| (φ.models φ.vars).product (s \ φ.vars).powerset := by
     intro ⟨v1, t1⟩ h21 ⟨v2, t2⟩ h22 h23
-    simp only [Set.mem_prod, mem_product, mem_coe, mem_models, Set.mem_preimage, mem_powerset, and_imp,
-      subset_sdiff, Prod.forall, Prod.mk.injEq] at h21 h22 h23 |-
+    simp only [Set.mem_prod, mem_product, mem_coe, mem_models, Set.mem_preimage, mem_powerset,
+      and_imp, subset_sdiff, Prod.forall, Prod.mk.injEq] at h21 h22 h23 |-
     constructor
     . ext x
       by_cases hx : x ∈ φ.vars
@@ -201,12 +283,109 @@ theorem card_models_vars {φ : PropForm ν} {s : Finset ν} (h : φ.vars ⊆ s) 
         rw [←toPropAssignment_eq_true, this, toPropAssignment_eq_true]
   rw [←h1, card_image_of_injOn h2, card_product, card_powerset, card_sdiff h]
 
-end PropForm
+theorem card_models_conj_aux {φ ψ: PropForm ν} (hdisj : φ.vars ∩ ψ.vars = ∅) :
+    card ((φ.conj ψ).models (φ.conj ψ).vars) =
+      card (φ.models φ.vars) * card (ψ.models ψ.vars) := by
+  let f (p : PropAssignment ν × PropAssignment ν) : PropAssignment ν :=
+    fun x => if x ∈ φ.vars then p.1 x else p.2 x
+  have h1 : ((φ.models φ.vars).product (ψ.models ψ.vars)).image f =
+    (φ.conj ψ).models (φ.vars ∪ ψ.vars) := by
+    ext v; simp [mem_image, mem_product, mem_models, Prod.exists, eval, Bool.and_eq_true]
+    constructor
+    . rintro ⟨v1, v2, ⟨⟨_, heval1⟩, ⟨hdef2, heval2⟩⟩, rfl⟩
+      constructor
+      . intro x hx
+        rw [mem_union, not_or] at hx
+        dsimp; rw [if_neg hx.1, hdef2 hx.2]
+      . constructor
+        . rw [←heval1]; apply eval_ext
+          intro x hx; rw [if_pos hx]
+        . rw [←heval2]; apply eval_ext
+          intro x hx
+          simp only [eq_empty_iff_forall_not_mem, mem_inter, not_and'] at hdisj
+          have hx' : x ∉ φ.vars := hdisj _ hx
+          rw [if_neg hx']
+    . intro ⟨hdef, heval1, heval2⟩
+      use fun x => if x ∈ φ.vars then v x else false
+      use fun x => if x ∈ ψ.vars then v x else false
+      dsimp
+      constructor
+      . constructor
+        . constructor
+          . intro x hx; dsimp; rw [if_neg hx]
+          . rw [←heval1]
+            apply eval_ext; intro x hx; rw [if_pos hx]
+        . constructor
+          . intro x hx; dsimp; rw [if_neg hx]
+          . rw [←heval2]
+            apply eval_ext; intro x hx; rw [if_pos hx]
+      . ext x
+        have := @hdef x
+        split <;> simp_all
+  have h2 : Set.InjOn f <| (φ.models φ.vars).product (ψ.models ψ.vars) := by
+    intro ⟨p11, p12⟩ hp1 ⟨p21, p22⟩ hp2
+    simp only [coe_product, Set.mem_prod, mem_coe, mem_models] at hp1 hp2
+    clear h1; revert f; dsimp; intro h
+    rw [Prod.mk.injEq]
+    constructor
+    . ext x
+      have := congr_fun h x
+      by_cases h' : x ∈ φ.vars <;> simp_all
+      rw [hp1.1.1 h', hp2.1.1 h']
+    . ext x
+      have := congr_fun h x
+      by_cases h' : x ∈ φ.vars <;> simp_all
+      simp only [eq_empty_iff_forall_not_mem, mem_inter, not_and] at hdisj
+      rw [hp1.2.1 (hdisj _ h'), hp2.2.1 (hdisj _ h')]
+  rw [vars, ←h1, card_image_of_injOn h2, card_product]
+
+@[simp] theorem card_models_conj {φ ψ : PropForm ν} {s : Finset ν}
+      (hsub : φ.vars ∪ ψ.vars ⊆ s) (hdisj : vars φ ∩ vars ψ = ∅) :
+    card ((φ.conj ψ).models s) = card (φ.models s) * card (ψ.models s) / 2^(card s):= by
+  symm; apply Nat.div_eq_of_eq_mul_left
+  . apply pow_pos; apply zero_lt_two
+  have hφ := union_subset_left hsub
+  have hψ := union_subset_right hsub
+  have card_un := card_disjoint_union (disjoint_iff_inter_eq_empty.mpr hdisj)
+  have aux : card (vars ψ) ≤ card s - card (vars φ) := by
+    apply Nat.le_sub_of_add_le
+    rw [add_comm, ←card_un]
+    exact card_le_of_subset hsub
+  have : (φ.conj ψ).vars ⊆ s := by rw [vars, union_subset_iff]; exact ⟨hφ, hψ⟩
+  rw [card_models_vars hφ, card_models_vars hψ, card_models_vars this, card_models_conj_aux hdisj]
+  rw [mul_right_comm]; simp only [mul_assoc, ←pow_add]
+  rw [←Nat.sub_add_comm (card_le_of_subset hψ)]
+  rw [Nat.add_sub_assoc aux, add_comm (card s)]
+  rw [vars, card_un, tsub_tsub]
 
 /-
 The main theorem.
 -/
 
-theorem countModels_eq_card_models {φ : PropForm ν} {s : Finset ν} (hvars : φ.vars ⊆ s) (hdec : φ.decomposable) :
+theorem countModels_eq_card_models {φ : PropForm ν} {s : Finset ν}
+      (hvars : φ.vars ⊆ s) (hdec : φ.decomposable) :
     φ.countModels s = card (φ.models s) := by
-  sorry
+  induction φ
+  case var x      =>
+    rw [vars, singleton_subset_iff] at hvars
+    rw [countModels, card_models_var hvars]
+  case tr         => simp [countModels]
+  case fls        => simp [countModels]
+  case neg φ ih   =>
+    rw [vars] at hvars
+    rw [decomposable] at hdec
+    rw [countModels, card_models_neg φ, ih hvars hdec]
+  case conj φ ψ ihφ ihψ =>
+    rw [vars] at hvars
+    have hφ := union_subset_left hvars
+    have hψ := union_subset_right hvars
+    rw [decomposable] at hdec
+    rw [countModels, card_models_conj hvars hdec.2.2, ihφ hφ hdec.1, ihψ hψ hdec.2.1]
+  case disj φ ψ ihφ ihψ =>
+    rw [vars, union_subset_iff] at hvars
+    rw [decomposable] at hdec
+    rw [countModels, card_models_disj_disjoint s hdec.2.2, ihφ hvars.1 hdec.1, ihψ hvars.2 hdec.2.1]
+  case impl  _    => rw [decomposable] at hdec; contradiction
+  case biImpl _ _ => rw [decomposable] at hdec; contradiction
+
+end PropForm
